Initial support for signatures modeling.
We provide an abstraction to verify signatures
by consulting with the trusted network entity in
the system, which keeps track of all messages and
can detect when a host has tried to impersonate an
other peer host.

network.s.dfy
@@ -27,6 +27,9 @@ module HostIdentifiers {
 // the Message type before the Network module. (Contrast with ch05/ex02.)
 module Network {
   import opened Library
+  import opened HostIdentifiers
+
+  datatype Message<Payload(==)> = Message(sender:HostId, payload:Payload)
 
   // A MessageOps is a "binding variable" used to connect a Host's Next step
   // (what message got received, what got sent?) with the Network (only allow
@@ -34,7 +37,9 @@ module Network {
   // Note that both fields are Option. A step predicate can say recv.None?
   // to indicate that it doesn't need to receive a message to occur.
   // It can say send.None? to indicate that it doesn't want to transmit a message.
-  datatype MessageOps<Message> = MessageOps(recv:Option<Message>, send:Option<Message>) {
+  datatype MessageOps<Payload> = MessageOps(recv:Option<Message<Payload>>, 
+                                            send:Option<Message<Payload>>,
+                                            signatureChecks:set<Message<Payload>>) {
     predicate IsSend()
     {
       && recv.None?
@@ -54,19 +59,26 @@ module Network {
   // allow it to be delivered over and over.
   // (We don't have packet headers, so duplication, besides being realistic,
   // also doubles as how multiple parties can hear the message.)
-  datatype Variables<Message> = Variables(sentMsgs:set<Message>)
+  datatype Variables<Payload> = Variables(correctlySignedMsgs:set<Message<Payload>>,
+                                                   sentMsgs:set<Message<Payload>>)
 
-  predicate Init<Message>(c: Constants, v: Variables<Message>)
+  predicate Init(c: Constants, v: Variables)
   {
     && v.sentMsgs == {}
+    && v.correctlySignedMsgs == {}
   }
 
-  predicate Next<Message>(c: Constants, v: Variables, v': Variables, msgOps: MessageOps)
+  predicate Next(c: Constants, v: Variables, v': Variables, msgOps: MessageOps, sender:HostId)
   {
     // Only allow receipt of a message if we've seen it has been sent.
     && (msgOps.recv.Some? ==> msgOps.recv.value in v.sentMsgs)
     // Record the sent message, if there was one.
-    && v'.sentMsgs ==
-      v.sentMsgs + if msgOps.send.None? then {} else { msgOps.send.value }
+    && (v'.sentMsgs ==
+        v.sentMsgs + if msgOps.send.Some? then { msgOps.send.value } else {})
+    && (v'.correctlySignedMsgs == v.correctlySignedMsgs 
+                                 + if msgOps.send.Some? && msgOps.send.value.sender == sender
+                                 then {msgOps.send.value} 
+                                 else {})
+    && msgOps.signatureChecks <= v.correctlySignedMsgs
   }
 }
